src/Helpers/RelationAlgebra.v
@@ -1284,6 +1284,10 @@ Module RelationNotations.
                               (at level 20, p1 at level 100, p2 at level 200, right associativity,
                                format "'[' x  <-  '[v    ' p1 ']' ; ']'  '/' p2")
                              : relation_scope.
+  Notation "'let!' x <- p1 ; p2" := (and_then p1 (fun x => p2))
+                              (at level 20, x pattern, p1 at level 100, p2 at level 200, right associativity,
+                               format "'[' 'let!' x  <-  '[v    ' p1 ']' ; ']'  '/' p2")
+                             : relation_scope.
   Ltac destruct_return :=
     match goal with
     | [ y : Return _ _  |- _ ] => destruct y
